vstep/lock_spec_automation.v
@@ -1,0 +1,174 @@
+(* Require Import VST.vstep.vstep. *)
+From diaframe Require Import defs proofmode_base util_classes.
+From VST.atomics Require Import general_atomics verif_lock_atomic.
+Require Import VST.floyd.library.
+From  VST.concurrency Require Import threads lock_specs.
+
+Section DVST_LOCK_SPECS.
+
+  (* #[local] Instance CompSpecs : compspecs. make_compspecs prog. Defined.
+  Definition Vprog : varspecs. mk_varspecs prog. Defined. *)
+
+  Context `{!VSTGS OK_ty Σ}.
+   (*
+  Lemma make_lock_inv_1' : forall v N, 
+    atomic_int_at Ews (vint 1) v ⊢
+      ∀ R, |={⊤}=> (∃ h, <affine> ⌜ptr_of h = v /\ name_of h = N⌝ ∗ lock_inv 1 h (R h)).
+    Proof.
+      intros.
+      iIntros "a".
+      iDestruct (atomic_int_isptr with "a") as %Ha.
+      iMod cinv_alloc_strong as (g) "(_ & Hg & Hi)"; first apply pred_infinite_True.
+      iIntros (h).
+      iExists (v, N, g); unfold lock_inv; simpl; iFrame.
+      iMod ("Hi" $! (inv_for_lock v (h (v, N, g))) with "[-]").
+    { iExists true; iFrame; done. }
+      iModIntro; iSplit. done. iSplit; done.
+    Qed.
+    (* lock specs that defers committing to a certain invariant *)
+  Program Definition makelock_spec_inv_defered :=
+  WITH gv: _, N : _
+  PRE [ ]
+     PROP ()
+     PARAMS () GLOBALS (gv)
+     SEP (mem_mgr gv)
+  POST [ tptr t_lock ] (* asymmetric consequence makes this messy *) ∃ v,
+     PROP ()
+     RETURN (v)
+     SEP (mem_mgr gv;  ∀ R, |={⊤}=> ∃ h , <affine> ⌜ptr_of h = v /\ name_of h = N⌝ ∗ lock_inv 1 h (R h)).
+
+  Lemma makelock_inv_defered: funspec_sub (snd makelock_spec) makelock_spec_inv_defered.
+  Proof.
+    split; first done. intros (gv, N) ?; simpl in *. Intros.
+    iIntros "H !>". iExists gv, emp. rewrite bi.emp_sep. iSplit; first done; iSplit; auto.
+    iPureIntro. intros. Intros. rewrite bi.emp_sep. monPred.unseal. Intros x; Exists x.
+    iIntros "(? & $ & $ & H & _)".
+    iSplit; first done.
+    rewrite bi.sep_emp. iApply make_lock_inv_1'.
+    iFrame. 
+  Qed.
+
+  Lemma and_affine_sep {prop:bi} P (Q:prop) :
+    Persistent P -> Absorbing P ->
+      P ∧ Q ⊣⊢ <affine> P ∗ Q.
+  Proof. intros; iSplit; iIntros "[? ?]"; iFrame. Qed.
+
+  Program Definition release_inv_spec_defered :=
+    WITH h : _
+    PRE [ tptr t_lock ]
+       PROP ()
+       PARAMS (ptr_of h)
+       SEP (∀ R, lock_inv 1 h R)
+    POST [ tvoid ]
+       PROP ()
+       LOCAL ()
+       SEP (∀ R, R -∗ lock_inv 1 h R).
+
+  Lemma release_inv_defered : funspec_sub (snd release_spec) release_inv_spec_defered.
+  Proof.
+    split; first done. intros h ?. simpl in *. Intros.
+    unfold rev_curry, tcurry. iIntros "H !>".
+    destruct h as ((v, N), g).
+    iExists (v, emp), emp. simpl in *.
+    rewrite bi.emp_sep. iSplit; first done; iSplit.
+    - unfold PROPx, PARAMSx, GLOBALSx, LOCALx, SEPx, argsassert2assert; simpl; monPred.unseal.
+      iDestruct "H" as "(_ & % & _ & H)".
+      do 4 (iSplit; auto).
+      iDestruct "H" as "(H & _)".
+      unfold lock_inv; simpl; unfold atomic_lock_inv.
+      (* iDestruct "H2" as "(% & #H & H2)". *)
+      (* rewrite -> prop_true_andp by auto. *)
+      unfold atomic_shift. iAuIntro. unfold atomic_acc; simpl.
+      admit.
+    - iPureIntro. iIntros (rho') "[% _]".
+      unfold PROPx, LOCALx, SEPx; simpl. rewrite bi.sep_emp //.
+
+      iSplit; [done|].
+      iSplit; [done|].
+      iIntros.
+      unfold lock_inv. unfold atomic_impl.
+      unfold atomic_lock_inv.
+  Admitted.
+
+ *)
+
+  Context {LI : lock_impl}.
+
+  Notation InvType := Mpred.
+  
+  Program Definition release_spec_simple :=
+    TYPE (ProdType (ConstType _) InvType)
+    WITH sh : _, h : _, R : _
+    PRE [ tptr t_lock ]
+       PROP ()
+       PARAMS (ptr_of h)
+       SEP (lock_inv sh h R; <affine> ⌜ExclusiveProp R⌝; R)
+    POST [ tvoid ]
+       PROP ()
+       LOCAL ()
+       SEP (lock_inv sh h R).
+  Next Obligation.
+  Admitted.
+  
+  Lemma release_simple : funspec_sub release_spec release_spec_simple.
+  Proof.
+    unfold funspec_sub; simpl.
+    split; first done; intros ((sh, h), R) ?; Intros.
+    iIntros "(? & ? & H) !>"; iExists (sh, h, R, R, lock_inv sh h R), emp.
+    iSplit; first done.
+    iSplit; last by iPureIntro; entailer!.
+    repeat (iSplit; first done).
+    rewrite /SEPx /= /LOCALx /argsassert2assert /=; monPred.unseal.
+    repeat (iSplit; first done).
+    iDestruct "H" as "(? & HR & % & ? & _)".
+    iSplitR.
+    { rewrite H0; done. }
+    iFrame; auto.
+  Qed.
+
+ Program Definition freelock_spec_simple :=
+    TYPE (ProdType (ConstType _) InvType)
+    WITH h : _, R : _
+    PRE [ tptr t_lock ]
+     PROP ()
+     PARAMS (ptr_of h)
+     SEP (lock_inv 1 h R; <affine> ⌜ExclusiveProp R⌝; R)
+   POST[ tvoid ]
+     PROP ()
+     LOCAL ()
+     SEP (R).
+  Next Obligation.
+  Admitted.
+  
+  Lemma freelock_simple : funspec_sub freelock_spec freelock_spec_simple.
+  Proof.
+    unfold funspec_sub; simpl.
+    split; first done; intros (h, R) ?; Intros.
+    iIntros "(? & ? & H) !>"; iExists (h, R, R), emp.
+    iSplit; first done.
+    iSplit; last by iPureIntro; entailer!.
+    repeat (iSplit; first done).
+    rewrite /SEPx /= /LOCALx /argsassert2assert /=; monPred.unseal.
+    repeat (iSplit; first done).
+    iDestruct "H" as "(? & $ & %HR & ? & _)".
+    iFrame; rewrite bi.sep_emp.
+    iModIntro.
+    iIntros " (r1 & ? & r2)".
+    iPoseProof (HR with "[r1 r2]") as "?"; iFrame.
+  Qed.
+
+End DVST_LOCK_SPECS.
+
+(* name of function (an AST.ident), a list of spec subsume relations to try  *)
+Ltac2 Type vstep_specs_type := (constr * constr) list.
+Ltac2 mutable vstep_specs : unit -> vstep_specs_type  := fun _ => [].
+
+Ltac2 Set vstep_specs as old_vstep_specs :=
+  fun _ => 
+            (constr:(_makelock), constr:(funspec_sub_refl_dep))::
+            (constr:(_freelock), constr:(freelock_simple))::
+            (constr:(_release), constr:(release_simple))::
+            (* (constr:(_release), constr:(release_simple2)):: *)
+            (constr:(_acquire), constr:(funspec_sub_refl_dep))::
+            (constr:(_spawn), constr:(funspec_sub_refl_dep))::
+            (old_vstep_specs ()).
